HittingSetToSetCover/HittingSetToSetCover_interfaces.dfy
@@ -8,7 +8,7 @@ method HittingSet_to_SetCover_Method(U:Set<int>, S:SetSet<int>, k: nat) returns 
   requires forall s | s in S.Model() ::  s <= U.Model()
   requires init_Set(U)
   requires init_SetSet(S)
-  requires S.maximumSizeElements() <= U.Size()
+  requires S.UBSize1() <= U.UBSize0()
   ensures (r.0.Model(),r.1.Model(),r.2) == HittingSet_to_SetCover(U.Model(), S.Model(), k)
   ensures counter <= poly(U, S, k)
 {
@@ -17,7 +17,7 @@ method HittingSet_to_SetCover_Method(U:Set<int>, S:SetSet<int>, k: nat) returns 
   var empty_set:Set<int>; empty_set, counter := New_Set(counter);
   var S_contains_empty:bool; S_contains_empty, counter := S.Contains(empty_set, counter);
   if (S_contains_empty) {
-    var SS:SetSetSet<int>; SS, counter := New_SetSetSet_params((set s | s in S.Model() :: {s}), S.maximumSizeElements(), U.Size(), counter);
+    var SS:SetSetSet<int>; SS, counter := New_SetSetSet_params((set s | s in S.Model() :: {s}), S.UBSize1(), U.UBSize0(), counter);
     var S':SetSet<int>; S', counter := S.Copy(counter);
     var S'_empty:bool; S'_empty, counter := S'.Empty(counter);
     while (!S'_empty)
@@ -28,17 +28,17 @@ method HittingSet_to_SetCover_Method(U:Set<int>, S:SetSet<int>, k: nat) returns 
       invariant U.Valid()
       invariant SS.Valid()
       invariant in_universe_SetSet(S', S)
-      invariant S.maximumSizeElements() <= U.Size()
+      invariant S.UBSize1() <= U.UBSize0()
       invariant SS.Cardinality() <= S.Cardinality() - S'.Cardinality()
-      invariant SS.maximumSizeElements() <= S.maximumSizeElements()
+      invariant SS.UBSize1() <= S.UBSize1()
       // Regular invariants
       invariant SS.Model() == (set s | s in (S.Model() - S'.Model()) :: {s})
       // Counter
-      invariant counter <= 2*S.Size() + 3 + (S.Cardinality() - S'.Cardinality())*(poly_edge_case_loop(U, S, k))
+      invariant counter <= 2*S.UBSize0() + 3 + (S.Cardinality() - S'.Cardinality())*(poly_edge_case_loop(U, S, k))
     {
       ghost var prevS' := S';
       S', SS, S'_empty, counter := HittingSet_to_SetCover_edge_case_loop(U, S, k, S', SS, counter);
-      assert counter <= 2*S.Size() + 3 + (S.Cardinality() - prevS'.Cardinality())*(poly_edge_case_loop(U, S, k)) + poly_edge_case_loop(U, S, k);
+      assert counter <= 2*S.UBSize0() + 3 + (S.Cardinality() - prevS'.Cardinality())*(poly_edge_case_loop(U, S, k)) + poly_edge_case_loop(U, S, k);
       calc == {
         (S.Cardinality() - prevS'.Cardinality())*(poly_edge_case_loop(U, S, k)) + poly_edge_case_loop(U, S, k);
         (S.Cardinality() - prevS'.Cardinality() + 1)*(poly_edge_case_loop(U, S, k));
@@ -49,7 +49,7 @@ method HittingSet_to_SetCover_Method(U:Set<int>, S:SetSet<int>, k: nat) returns 
     return (S, SS, 0), counter;
   }
   // Regular case
-  var SS:SetSetSet<int>; SS, counter := New_SetSetSet_params((set u | u in U.Model() :: (set s | s in S.Model() && u in s)), S.Size(), U.Size(), counter);
+  var SS:SetSetSet<int>; SS, counter := New_SetSetSet_params((set u | u in U.Model() :: (set s | s in S.Model() && u in s)), S.UBSize0(), U.UBSize0(), counter);
   var U':Set<int>; U', counter := U.Copy(counter);
   var U'_empty:bool; U'_empty, counter := U'.Empty(counter);
   while (!U'_empty)
@@ -60,15 +60,15 @@ method HittingSet_to_SetCover_Method(U:Set<int>, S:SetSet<int>, k: nat) returns 
     invariant SS.Valid()
     invariant in_universe_Set(U', U)
     invariant SS.Cardinality() <= U.Cardinality() - U'.Cardinality()
-    invariant SS.maximumSizeElements() <= S.Size()
+    invariant SS.UBSize1() <= S.UBSize0()
     // Regular invariants
     invariant SS.Model() == (set u | u in (U.Model() - U'.Model()) :: (set s | s in S.Model() && u in s))
     // Counter
-    invariant counter <= S.Size() + U.Size() + 3 + (U.Cardinality() - U'.Cardinality())*poly_outer_loop(U, S, k)
+    invariant counter <= S.UBSize0() + U.UBSize0() + 3 + (U.Cardinality() - U'.Cardinality())*poly_outer_loop(U, S, k)
   {
     U', SS, U'_empty, counter := HittingSet_to_SetCover_outer_loop(U, S, k, U', SS, counter);
   }
-  assert counter <= S.Size() + U.Size() + 3 + U.Cardinality()*poly_outer_loop(U, S, k);
+  assert counter <= S.UBSize0() + U.UBSize0() + 3 + U.Cardinality()*poly_outer_loop(U, S, k);
   identity_substraction_lemma(U.Model(), U'.Model());
 
   return (S,SS,k),counter;
@@ -82,9 +82,9 @@ method HittingSet_to_SetCover_outer_loop(U:Set<int>, S:SetSet<int>, k:nat, U':Se
   requires S.Valid()
   requires SS.Valid()
   requires in_universe_Set(U', U)
-  requires S.maximumSizeElements() <= U.Size()
+  requires S.UBSize1() <= U.UBSize0()
   requires SS.Cardinality() <= (U.Cardinality() - U'.Cardinality())
-  requires SS.maximumSizeElements() <= S.Size()
+  requires SS.UBSize1() <= S.UBSize0()
   // Invariant in
   requires SS.Model() == (set u | u in (U.Model() - U'.Model()) :: (set s | s in S.Model() && u in s))
   // Termination out
@@ -94,7 +94,7 @@ method HittingSet_to_SetCover_outer_loop(U:Set<int>, S:SetSet<int>, k:nat, U':Se
   ensures SS'.Valid()
   ensures in_universe_Set(U'', U)
   ensures SS'.Cardinality() <= (U.Cardinality() - U''.Cardinality())
-  ensures SS'.maximumSizeElements() <= S.Size()
+  ensures SS'.UBSize1() <= S.UBSize0()
   // Invariant out
   ensures SS'.Model() == (set u | u in (U.Model() - U''.Model()) :: (set s | s in S.Model() && u in s))
   // Counter
@@ -105,7 +105,7 @@ method HittingSet_to_SetCover_outer_loop(U:Set<int>, S:SetSet<int>, k:nat, U':Se
   var u:int; u, counter := U'.Pick(counter);
   U'', counter := U'.Remove(u, counter);
 
-  var sets_in_S_that_contain_u:SetSet<int>; sets_in_S_that_contain_u, counter := New_SetSet_params(S.Model(), S.maximumSizeElements(), counter);
+  var sets_in_S_that_contain_u:SetSet<int>; sets_in_S_that_contain_u, counter := New_SetSet_params(S.Model(), S.UBSize1(), counter);
   var S'; S', counter := S.Copy(counter);
   var S'_empty; S'_empty, counter := S'.Empty(counter);
   while (!S'_empty)
@@ -116,11 +116,11 @@ method HittingSet_to_SetCover_outer_loop(U:Set<int>, S:SetSet<int>, k:nat, U':Se
     invariant U.Valid()
     invariant in_universe_SetSet(S', S)
     invariant in_universe_SetSet(sets_in_S_that_contain_u, S)
-    invariant S.maximumSizeElements() <= U.Size()
+    invariant S.UBSize1() <= U.UBSize0()
     // Regular invariants
     invariant sets_in_S_that_contain_u.Model() == (set s | s in (S.Model() - S'.Model()) && u in s)
     // Counter
-    invariant counter <= counter_in + S.Size() + U.Size() + 3 + (S.Cardinality() - S'.Cardinality())*(poly_middle_loop(U, S, k))
+    invariant counter <= counter_in + S.UBSize0() + U.UBSize0() + 3 + (S.Cardinality() - S'.Cardinality())*(poly_middle_loop(U, S, k))
   {
     ghost var S'_prev := S';
     S', sets_in_S_that_contain_u, S'_empty, counter := HittingSet_to_SetCover_middle_loop(U, S, k, S', u, sets_in_S_that_contain_u, counter);
@@ -130,7 +130,7 @@ method HittingSet_to_SetCover_outer_loop(U:Set<int>, S:SetSet<int>, k:nat, U':Se
   SS', counter := SS.Add(sets_in_S_that_contain_u, counter);
 
   U''_empty, counter := U''.Empty(counter);
-  mult_preserves_order(SS.Cardinality(), SS.maximumSizeElements(), U.Cardinality(), S.Size());
+  mult_preserves_order(SS.Cardinality(), SS.UBSize1(), U.Cardinality(), S.UBSize0());
   assert SS'.Model() == (set v | v in (U.Model() - U''.Model()) :: (set s | s in S.Model() && v in s)) by {
     assert SS'.Model() == (set v | v in (U.Model() - U'.Model()) :: (set s | s in S.Model() && v in s)) + {sets_in_S_that_contain_u.Model()};
     assert SS'.Model() == (set v | v in (U.Model() - U'.Model()) :: (set s | s in S.Model() && v in s)) + {(set s | s in (S.Model() - S'.Model()) && u in s)};
@@ -149,8 +149,8 @@ method HittingSet_to_SetCover_middle_loop(U:Set<int>, S:SetSet<int>, k:nat, S':S
   requires U.Valid()
   requires in_universe_SetSet(S', S)
   requires in_universe_SetSet(sets_in_S_that_contain_u, S)
-  requires S.maximumSizeElements() <= U.Size()
-  ensures sets_in_S_that_contain_u.Size() <= S.Size()
+  requires S.UBSize1() <= U.UBSize0()
+  ensures sets_in_S_that_contain_u.UBSize0() <= S.UBSize0()
   // Invariant in
   requires sets_in_S_that_contain_u.Model() == (set s | s in (S.Model() - S'.Model()) && u in s)
   // Termination out
@@ -182,21 +182,21 @@ method HittingSet_to_SetCover_middle_loop(U:Set<int>, S:SetSet<int>, k:nat, S':S
     // Types
     invariant s'.Valid()
     invariant in_universe_Set(s', s)
-    invariant s.Cardinality() <= S.maximumSizeElements()
-    invariant S.maximumSizeElements() <= U.Size()
+    invariant s.Cardinality() <= S.UBSize1()
+    invariant S.UBSize1() <= U.UBSize0()
     // Regular invariants
     invariant s_contains_u == (u in (s.Model() - s'.Model()))
     // Counter
-    invariant counter <= counter_in + 2*S.Size() + 2*U.Size() + 1 + (s.Cardinality() - s'.Cardinality())*poly_inner_loop(U, S, k)
+    invariant counter <= counter_in + 2*S.UBSize0() + 2*U.UBSize0() + 1 + (s.Cardinality() - s'.Cardinality())*poly_inner_loop(U, S, k)
   {
     s', s_contains_u, s'_empty, counter := HittingSet_to_SetCover_inner_loop(U, S, k, s, s', u, s_contains_u, counter);
   }
-  mult_preserves_order(s.Cardinality(), poly_inner_loop(U, S, k), U.Size(), poly_inner_loop(U, S, k));
+  mult_preserves_order(s.Cardinality(), poly_inner_loop(U, S, k), U.UBSize0(), poly_inner_loop(U, S, k));
   if (s_contains_u) {
     sets_in_S_that_contain_u', counter := sets_in_S_that_contain_u.Add(s, counter);
   }
   S''_empty, counter := S''.Empty(counter);
-  assert counter <= counter_in + 3*S.Size() + 2*U.Size() + 2 + U.Size()*poly_inner_loop(U, S, k);
+  assert counter <= counter_in + 3*S.UBSize0() + 2*U.UBSize0() + 2 + U.UBSize0()*poly_inner_loop(U, S, k);
 }
 
 method HittingSet_to_SetCover_inner_loop(U:Set<int>, S:SetSet<int>, k:nat, s:Set<int>, s':Set<int>, u:int, s_contains_u:bool, ghost counter_in:nat) returns (s'':Set<int>, s_contains_u':bool, s''_empty:bool, ghost counter:nat)
@@ -206,8 +206,8 @@ method HittingSet_to_SetCover_inner_loop(U:Set<int>, S:SetSet<int>, k:nat, s:Set
   requires U.Valid()
   requires S.Valid()
   requires in_universe_Set(s', s)
-  requires s.Cardinality() <= S.maximumSizeElements()
-  requires S.maximumSizeElements() <= U.Size()
+  requires s.Cardinality() <= S.UBSize1()
+  requires S.UBSize1() <= U.UBSize0()
   // Invariant in
   requires s_contains_u == (u in (s.Model() - s'.Model()))
   // Termination out
@@ -239,14 +239,14 @@ requires S'.Model() != {}
 // Types in
 requires U.Valid()
 requires in_universe_SetSet(S', S)
-requires S.maximumSizeElements() <= U.Size()
+requires S.UBSize1() <= U.UBSize0()
 // Invariant in
 requires S_contains_empty == ({} in (S.Model() - S'.Model()))
 // Termination out
 ensures S''.Cardinality() == S'.Cardinality() - 1
 // Types out
 ensures in_universe_SetSet(S'', S)
-ensures S''.maximumSizeElements() <= U.Size()
+ensures S''.UBSize1() <= U.UBSize0()
 // Invariant out
 ensures S_contains_empty'== ({} in (S.Model() - S''.Model()))
 // Counter
@@ -268,9 +268,9 @@ method HittingSet_to_SetCover_edge_case_loop(U:Set<int>, S:SetSet<int>, k:nat, S
   requires U.Valid()
   requires SS.Valid()
   requires in_universe_SetSet(S', S)
-  requires S.maximumSizeElements() <= U.Size()
+  requires S.UBSize1() <= U.UBSize0()
   requires SS.Cardinality() <= S.Cardinality() - S'.Cardinality()
-  requires SS.maximumSizeElements() <= S.maximumSizeElements()
+  requires SS.UBSize1() <= S.UBSize1()
   // Invariant in
   requires SS.Model() == (set s | s in (S.Model() - S'.Model()) :: {s})
   // Termination out
@@ -280,18 +280,18 @@ method HittingSet_to_SetCover_edge_case_loop(U:Set<int>, S:SetSet<int>, k:nat, S
   ensures SS'.Valid()
   ensures in_universe_SetSet(S'', S)
   ensures SS'.Cardinality() <= S.Cardinality() - S''.Cardinality()
-  ensures SS'.maximumSizeElements() <= S.maximumSizeElements()
+  ensures SS'.UBSize1() <= S.UBSize1()
   // Invariant out
   ensures SS'.Model() == (set s | s in (S.Model() - S''.Model()) :: {s})
   // Counter
   ensures counter <= counter_in + poly_edge_case_loop(U, S, k)
 {
   in_universe_lemma_SetSet(S', S);
-  mult_preserves_order(SS.Cardinality(), SS.maximumSizeElements(), S.Cardinality(), S.maximumSizeElements());
+  mult_preserves_order(SS.Cardinality(), SS.UBSize1(), S.Cardinality(), S.UBSize1());
   counter := counter_in;
   var s:Set<int>; s, counter := S'.Pick(counter);
   S'', counter := S'.Remove(s, counter);
-  var s_set:SetSet<int>; s_set, counter := New_SetSet_params(S.Model(), S.maximumSizeElements(), counter);
+  var s_set:SetSet<int>; s_set, counter := New_SetSet_params(S.Model(), S.UBSize1(), counter);
   s_set, counter := s_set.Add(s, counter);
   SS', counter := SS.Add(s_set, counter);
   S''_empty, counter := S''.Empty(counter);
@@ -300,58 +300,58 @@ method HittingSet_to_SetCover_edge_case_loop(U:Set<int>, S:SetSet<int>, k:nat, S
 
 lemma counter_simplification_aux_1(U: Set<int>, S: SetSet<int>, k: nat, S'_prev: SetSet<int>, S': SetSet<int>)
   requires S'_prev.Cardinality() == S'.Cardinality() + 1
-  ensures S.Size() + U.Size() + 3 + (S.Cardinality() - S'_prev.Cardinality())*(poly_middle_loop(U, S, k)) + poly_middle_loop(U, S, k) ==
-          S.Size() + U.Size() + 3 + (S.Cardinality() - S'.Cardinality())*(poly_middle_loop(U, S, k))
+  ensures S.UBSize0() + U.UBSize0() + 3 + (S.Cardinality() - S'_prev.Cardinality())*(poly_middle_loop(U, S, k)) + poly_middle_loop(U, S, k) ==
+          S.UBSize0() + U.UBSize0() + 3 + (S.Cardinality() - S'.Cardinality())*(poly_middle_loop(U, S, k))
 {}
 
 
 ghost function poly_inner_loop(U: Set<int>, S: SetSet<int>, k: nat) : (o:nat)
 {
-  U.Size() + 2
+  U.UBSize0() + 2
 }
 ghost function poly_middle_loop(U: Set<int>, S: SetSet<int>, k: nat) : (o:nat)
-  ensures 3*S.Size() + 2*U.Size() + 2 + U.Size()*poly_inner_loop(U, S, k) <= o
+  ensures 3*S.UBSize0() + 2*U.UBSize0() + 2 + U.UBSize0()*poly_inner_loop(U, S, k) <= o
 {
   /*calc <= {
-    3*S.Size() + 2*U.Size() + 2 + U.Size()*poly_inner_loop(U, S, k);
-    3*S.Size() + 2*U.Size() + 2 + U.Size()*(U.Size() + 2);
-    3*S.Size() + 2*U.Size() + 2 + U.Size()*U.Size() + 2*U.Size();
-    U.Size()*U.Size() + 3*S.Size() + 4*U.Size() + 1;
+    3*S.UBSize0() + 2*U.UBSize0() + 2 + U.UBSize0()*poly_inner_loop(U, S, k);
+    3*S.UBSize0() + 2*U.UBSize0() + 2 + U.UBSize0()*(U.UBSize0() + 2);
+    3*S.UBSize0() + 2*U.UBSize0() + 2 + U.UBSize0()*U.UBSize0() + 2*U.UBSize0();
+    U.UBSize0()*U.UBSize0() + 3*S.UBSize0() + 4*U.UBSize0() + 1;
   }*/
-  U.Size()*U.Size() + 3*S.Size() + 4*U.Size() + 2
+  U.UBSize0()*U.UBSize0() + 3*S.UBSize0() + 4*U.UBSize0() + 2
 }
 ghost function poly_outer_loop(U: Set<int>, S: SetSet<int>, k: nat) : (o:nat)
-  ensures S.Size() + U.Size() + 4 + S.Cardinality()*(poly_middle_loop(U, S, k)) + S.Size()*U.Cardinality() <= o
+  ensures S.UBSize0() + U.UBSize0() + 4 + S.Cardinality()*(poly_middle_loop(U, S, k)) + S.UBSize0()*U.Cardinality() <= o
 {
   /*calc <= {
-    S.Size() + U.Size() + 4 + S.Cardinality()*(poly_middle_loop(U, S, k)) + S.Size()*U.Cardinality();
-    S.Size()*U.Cardinality() + S.Size() + U.Size() + 4 + S.Cardinality()*(poly_middle_loop(U, S, k));
-    S.Size()*U.Cardinality() + S.Size() + U.Size() + 4 + S.Cardinality()*(U.Size()*U.Size() + 3*S.Size() + 4*U.Size() + 2);
-    S.Size()*U.Cardinality() + S.Size() + U.Size() + 4 + (U.Size()*U.Size()*S.Cardinality() + 3*S.Size()*S.Cardinality() + 4*U.Size()*S.Cardinality() + 2*S.Cardinality());
-    U.Size()*U.Size()*S.Cardinality() + 3*S.Size()*S.Cardinality() + S.Size()*U.Cardinality() + 4*U.Size()*S.Cardinality() + S.Size() + U.Size() + 2*S.Cardinality() + 4;
+    S.UBSize0() + U.UBSize0() + 4 + S.Cardinality()*(poly_middle_loop(U, S, k)) + S.UBSize0()*U.Cardinality();
+    S.UBSize0()*U.Cardinality() + S.UBSize0() + U.UBSize0() + 4 + S.Cardinality()*(poly_middle_loop(U, S, k));
+    S.UBSize0()*U.Cardinality() + S.UBSize0() + U.UBSize0() + 4 + S.Cardinality()*(U.UBSize0()*U.UBSize0() + 3*S.UBSize0() + 4*U.UBSize0() + 2);
+    S.UBSize0()*U.Cardinality() + S.UBSize0() + U.UBSize0() + 4 + (U.UBSize0()*U.UBSize0()*S.Cardinality() + 3*S.UBSize0()*S.Cardinality() + 4*U.UBSize0()*S.Cardinality() + 2*S.Cardinality());
+    U.UBSize0()*U.UBSize0()*S.Cardinality() + 3*S.UBSize0()*S.Cardinality() + S.UBSize0()*U.Cardinality() + 4*U.UBSize0()*S.Cardinality() + S.UBSize0() + U.UBSize0() + 2*S.Cardinality() + 4;
   }*/
-  U.Size()*U.Size()*S.Cardinality() + 3*S.Size()*S.Cardinality() + S.Size()*U.Cardinality() + 4*U.Size()*S.Cardinality() + S.Size() + U.Size() + 2*S.Cardinality() + 4
+  U.UBSize0()*U.UBSize0()*S.Cardinality() + 3*S.UBSize0()*S.Cardinality() + S.UBSize0()*U.Cardinality() + 4*U.UBSize0()*S.Cardinality() + S.UBSize0() + U.UBSize0() + 2*S.Cardinality() + 4
 }
 ghost function poly_edge_case_loop(U: Set<int>, S: SetSet<int>, k: nat) : (o:nat)
 {
-  2*S.Size() + 2*U.Size() + 2
+  2*S.UBSize0() + 2*U.UBSize0() + 2
 }
 
 ghost function poly(U: Set<int>, S: SetSet<int>, k: nat) : (o:nat)
-  ensures 2*S.Size() + 3 + S.Cardinality()*poly_edge_case_loop(U, S, k) <= o           // If S contains empty
-  ensures S.Size() + U.Size() + 3 + U.Cardinality()*poly_outer_loop(U, S, k) <= o      // Otherwise
+  ensures 2*S.UBSize0() + 3 + S.Cardinality()*poly_edge_case_loop(U, S, k) <= o           // If S contains empty
+  ensures S.UBSize0() + U.UBSize0() + 3 + U.Cardinality()*poly_outer_loop(U, S, k) <= o      // Otherwise
 {
   calc == {
-    2*S.Size() + 3 + S.Cardinality()*(poly_edge_case_loop(U, S, k));
-    2*S.Size() + 3 + S.Cardinality()*(2*S.Size() + 2*U.Size() + 2);
-    2*S.Size() + 3 + (2*S.Size()*S.Cardinality() + 2*U.Size()*S.Cardinality() + 2*S.Cardinality());
-    2*S.Size()*S.Cardinality() + 2*U.Size()*S.Cardinality() + 2*S.Size() + 2*S.Cardinality() + 3;
+    2*S.UBSize0() + 3 + S.Cardinality()*(poly_edge_case_loop(U, S, k));
+    2*S.UBSize0() + 3 + S.Cardinality()*(2*S.UBSize0() + 2*U.UBSize0() + 2);
+    2*S.UBSize0() + 3 + (2*S.UBSize0()*S.Cardinality() + 2*U.UBSize0()*S.Cardinality() + 2*S.Cardinality());
+    2*S.UBSize0()*S.Cardinality() + 2*U.UBSize0()*S.Cardinality() + 2*S.UBSize0() + 2*S.Cardinality() + 3;
   }
   calc == {
-    S.Size() + U.Size() + 3 + U.Cardinality()*poly_outer_loop(U, S, k);
-    S.Size() + U.Size() + 3 + U.Cardinality()*(U.Size()*U.Size()*S.Cardinality() + 3*S.Size()*S.Cardinality() + S.Size()*U.Cardinality() + 4*U.Size()*S.Cardinality() + S.Size() + U.Size() + 2*S.Cardinality() + 4);
-    S.Size() + U.Size() + 3 + (U.Size()*U.Size()*S.Cardinality()*U.Cardinality() + 3*S.Size()*S.Cardinality()*U.Cardinality() + S.Size()*U.Cardinality()*U.Cardinality() + 4*U.Size()*S.Cardinality()*U.Cardinality() + S.Size()*U.Cardinality() + U.Size()*U.Cardinality() + 2*S.Cardinality()*U.Cardinality() + 4*U.Cardinality());
-    U.Size()*U.Size()*S.Cardinality()*U.Cardinality() + 3*S.Size()*S.Cardinality()*U.Cardinality() + S.Size()*U.Cardinality()*U.Cardinality() + 4*U.Size()*S.Cardinality()*U.Cardinality() + S.Size()*U.Cardinality() + U.Size()*U.Cardinality() + 2*S.Cardinality()*U.Cardinality() + S.Size() + U.Size() + 4*U.Cardinality() + 3;
+    S.UBSize0() + U.UBSize0() + 3 + U.Cardinality()*poly_outer_loop(U, S, k);
+    S.UBSize0() + U.UBSize0() + 3 + U.Cardinality()*(U.UBSize0()*U.UBSize0()*S.Cardinality() + 3*S.UBSize0()*S.Cardinality() + S.UBSize0()*U.Cardinality() + 4*U.UBSize0()*S.Cardinality() + S.UBSize0() + U.UBSize0() + 2*S.Cardinality() + 4);
+    S.UBSize0() + U.UBSize0() + 3 + (U.UBSize0()*U.UBSize0()*S.Cardinality()*U.Cardinality() + 3*S.UBSize0()*S.Cardinality()*U.Cardinality() + S.UBSize0()*U.Cardinality()*U.Cardinality() + 4*U.UBSize0()*S.Cardinality()*U.Cardinality() + S.UBSize0()*U.Cardinality() + U.UBSize0()*U.Cardinality() + 2*S.Cardinality()*U.Cardinality() + 4*U.Cardinality());
+    U.UBSize0()*U.UBSize0()*S.Cardinality()*U.Cardinality() + 3*S.UBSize0()*S.Cardinality()*U.Cardinality() + S.UBSize0()*U.Cardinality()*U.Cardinality() + 4*U.UBSize0()*S.Cardinality()*U.Cardinality() + S.UBSize0()*U.Cardinality() + U.UBSize0()*U.Cardinality() + 2*S.Cardinality()*U.Cardinality() + S.UBSize0() + U.UBSize0() + 4*U.Cardinality() + 3;
   }
-  U.Size()*U.Size()*S.Cardinality()*U.Cardinality() + 3*S.Size()*S.Cardinality()*U.Cardinality() + S.Size()*U.Cardinality()*U.Cardinality() + 4*U.Size()*S.Cardinality()*U.Cardinality() + 2*S.Size()*S.Cardinality() + S.Size()*U.Cardinality() + 2*U.Size()*S.Cardinality() + U.Size()*U.Cardinality() + 2*S.Cardinality()*U.Cardinality() + 2*S.Size() + U.Size() + 2*S.Cardinality() + 4*U.Cardinality() + 3
+  U.UBSize0()*U.UBSize0()*S.Cardinality()*U.Cardinality() + 3*S.UBSize0()*S.Cardinality()*U.Cardinality() + S.UBSize0()*U.Cardinality()*U.Cardinality() + 4*U.UBSize0()*S.Cardinality()*U.Cardinality() + 2*S.UBSize0()*S.Cardinality() + S.UBSize0()*U.Cardinality() + 2*U.UBSize0()*S.Cardinality() + U.UBSize0()*U.Cardinality() + 2*S.Cardinality()*U.Cardinality() + 2*S.UBSize0() + U.UBSize0() + 2*S.Cardinality() + 4*U.Cardinality() + 3
 }
